\documentclass[floatfix,nofootinbib,superscriptaddress,fleqn]{revtex4}  
%\documentclass[aps,epsfig,tightlines,fleqn]{revtex4}
\usepackage[utf]{kotex}
\usepackage[HWP]{dhucs-interword}
\usepackage[dvips]{color}
\usepackage{graphicx}
\usepackage{bm}
%\usepackage{fancyhdr}
%\usepackage{dcolumn}
\usepackage{defcolor}
\usepackage{amsmath}
\usepackage{amsfonts}
\usepackage{amssymb}
\usepackage{amscd}
\usepackage{amsthm}
\usepackage[utf8]{inputenc}
 \usepackage{setspace}
%\pagestyle{fancy}

\begin{document}
\begin{align*}
  {g^\nu}_\alpha g_{\beta\mu}-{g^\nu}_\beta g_{\alpha\mu}
\end{align*}
\begin{align*}
  {\Delta\omega^\nu}_\mu\left({g^\nu}_\alpha \gamma_\beta-{g^\nu}_\beta \gamma_\alpha\right)
  &=-\frac{i}{4}\left({\Delta\omega^\nu}_\mu-{\Delta\omega_\mu}^\nu\right)
  \left[\gamma^\nu,\sigma_{\alpha\beta}\right]  \\
  &=-\frac{i}{2}{\Delta\omega^\nu}_\mu\left[\gamma^\nu,\sigma_{\alpha\beta}\right]
\end{align*}
\begin{align*}
  \Longrightarrow 2i\left({g^\nu}_\alpha \gamma_\beta-{g^\nu}_\beta \gamma_\alpha\right)
  =\left[\gamma^\nu,\sigma_{\alpha\beta}\right]
\end{align*}
\begin{align*}
  \sigma_{\alpha\beta}=\frac i2\left[\gamma_\alpha,\gamma_\beta\right]
\end{align*}
\begin{align*}
  {I^\nu}_\mu=
  \begin{pmatrix}
    0&-1&0&0  \\
    -1&0&0&0  \\
    0&0&0&0  \\
    0&0&0&0  \\
  \end{pmatrix},\,\,\,
  \left({I^\nu}_\mu\right)^2=
  \begin{pmatrix}
    1&0&0&0  \\
    0&1&0&0  \\
    0&0&0&0  \\
    0&0&0&0  \\
  \end{pmatrix}
\end{align*}
\begin{align*}
  {a^\nu}_\mu&\approx{g^\nu}_\mu+{\Delta\omega^\nu}_\mu  \\
  &={g^\nu}_\mu+\Delta\omega{I^\nu}_\mu
\end{align*}
\begin{align*}
  \left(x^\nu\right)'\approx& \left(g+\frac{\omega}{N}I\right)^\nu_{\alpha_1}
  \left(g+\frac{\omega}{N}I\right)^{\alpha_1}_{\alpha_2}\cdots
  \left(g+\frac{\omega}{N}I\right)^{\alpha_{N-1}}_{\alpha_N}x^{\alpha_N}  
  =\lim_{N\rightarrow\infty}\left(g+\frac{\omega}{N}I\right)^\nu_{\alpha_1}\cdots
  \left(g+\frac{\omega}{N}I\right)^{\alpha_{N-1}}_{\alpha_N}x^{\alpha_N}  \\
  =&\lim_{N\rightarrow\infty}
  {{\left(g+\frac{\omega}{N}I\right)^{N}}^\nu}_\mu x^{\alpha_N}
  ={\left(e^{\omega I}\right)^\nu}_\mu x^\mu  \\
  &={\left(\cosh\omega I+\sinh \omega I\right)^\nu}_\mu x^\mu
\end{align*}
\begin{align*}
  {\left(x^\nu\right)'=\left(\mathbb{I}-I^2+I^2\cosh \omega+I\cosh \omega \right)^\nu}_\mu x^\mu
\end{align*}
\begin{align*}
  \begin{pmatrix}
    {x^0}' \\
    {x^1}' \\
    {x^2}'\\
    {x^3}'\\
  \end{pmatrix}
  =
  \begin{pmatrix}
    \cosh \omega&-\sinh \omega&0&0  \\
    -\sinh \omega&\cosh \omega&0&0  \\
    0&0&1&0  \\
    0&0&0&1  \\
  \end{pmatrix}
  \begin{pmatrix}
    {x^0} \\
    {x^1} \\
    {x^2}\\
    {x^3}\\
  \end{pmatrix}
\end{align*}
\begin{align*}
  \psi'(x')&=S\psi(x)=\lim_{N\rightarrow \infty}\left(1-\frac{i}{4}\frac{\omega}{N}
  \sigma_{\mu\nu}{I_n}^{\mu\nu}\right)^N\psi(x) \\
  &=\exp{\left(-\frac{i}{4}\omega
  \sigma_{\mu\nu}{I_n}^{\mu\nu}\right)}\psi(x)
\end{align*}
\begin{align*}
  \psi'(x')=e^{-\frac{i}{4}\omega\left(
  \sigma_{01}{I}^{01}+\sigma_{10}{I}^{10}\right)}\psi(x)=e^{-\frac{i}{2}\omega\sigma_{01}}\psi(x)
\end{align*}
\begin{align*}
  {I^\nu}_\mu=\begin{pmatrix}
    0&0&0&0 \\
    0&0&1&0 \\
    0&-1&0&0 \\
    0&0&0&0 \\
  \end{pmatrix},  \,\,\,
  \psi'(x')=e^{-\frac{i}{2}\phi\sigma_{12}}\psi(x)
\end{align*}
\begin{align*}
  j^\mu(x)=c\psi^\dagger\gamma^0\gamma^\mu\psi,\,\,\,
  {j^\mu}'(x')=c\psi'^\dagger(x')\gamma^0\gamma^\mu\psi'(x')
\end{align*}
\begin{align*}
  {j^\mu}'(x')&=c\psi^\dagger(x)S^\dagger\gamma^0\gamma^\mu S\psi(x) \\
  &=c\psi^\dagger(x)\gamma^0S^{-1}\gamma^\mu S\psi(x)  \\
  &=c{a^\mu}_\nu\psi^\dagger(x)\gamma^0\gamma^\mu\psi(x)  \\
  &=c{a^\mu}_\nu j^\mu(x)
\end{align*}
\begin{align*}
  {a^\nu}_\mu\gamma^\mu = S^{-1}(a)\gamma^\nu S(a)\Longrightarrow
  {a^\nu}_\mu\gamma^\mu = P^{-1}\gamma^\nu P
\end{align*}
\begin{align*}
  {a^\nu}_\mu = \begin{pmatrix}
    1&0&0&0&  \\
    0&-1&0&0&  \\
    0&0&-1&0&  \\
    0&0&0&-1&  \\
  \end{pmatrix}
  =g^{\nu\mu}
\end{align*}
\begin{align*}
  &{a^\sigma}_\nu {a^\nu}_\mu\gamma^\mu=P^{-1}{a^\sigma}_\nu\gamma^\nu P,\,\,\,
  {a^\sigma}_\nu\gamma^\nu=g^{\sigma\sigma}\gamma^{\sigma}  \\\
  &\Longrightarrow P{g^\sigma}_\mu\gamma^\mu P^{-1}=g^{\sigma\sigma}\gamma^{\sigma} 
\end{align*}
\begin{align*}
  P=e^{i\phi}\gamma^0\Longrightarrow \psi'(x')=\psi(-x)=P=e^{i\phi}\gamma^0\psi(x)
\end{align*}
\begin{align*}
  &\Gamma^s=\mathbb{I},\,\,\,\Gamma^V_\mu=\gamma_\mu,\,\,\,\Gamma^T_{\mu\nu}=\sigma_{\mu\nu} \\
  &\Gamma^P=i\gamma^0\gamma^1\gamma^2\gamma^3=\gamma^5=\gamma_5,\,\,\,\Gamma^A_\mu\gamma_5\gamma_\mu
\end{align*}
\begin{align*}
  U(I) = \begin{pmatrix}
    1&0\\
    0&1\\
  \end{pmatrix},
  U(C_3)= \begin{pmatrix}
    -\frac12&\frac12\sqrt{3}  \\
    -\frac12\sqrt{3}&-\frac12  \\
  \end{pmatrix}  ,
  U(C_3^2)= \begin{pmatrix}
    -\frac12&-\frac12\sqrt{3}  \\
    \frac12\sqrt{3}&-\frac12  \\
  \end{pmatrix} ,\\
  U(C_2)= \begin{pmatrix}
    1&0  \\
    0&-1  \\
  \end{pmatrix},
  U(C_2')= \begin{pmatrix}
    -\frac12&\frac12\sqrt{3}  \\
    \frac12\sqrt{3}&\frac12  \\
  \end{pmatrix},
  U(C_2'')= \begin{pmatrix}
    -\frac12&-\frac12\sqrt{3}  \\
    -\frac12\sqrt{3}&\frac12  \\
  \end{pmatrix}
\end{align*}

\begin{align*}
  U(t) &= \left<\mathbf{x}\left|e^{-i(\mathbf{p}^2/2m)t}
  \right| \mathbf{x_0}\right> \\
  &=\int \frac{d^3p}{(2\pi)^3}\left<\mathbf{x}\left|e^{-i(\mathbf{p}^2/2m)t}
  \right| \mathbf{p}\right>\left<\mathbf{p}|\mathbf{x_0}\right> \\
  &=\frac{1}{(2\pi)^3}\int d^3p e^{-i(\mathbf{p}^2/2m)t}\cdot
  e^{i\mathbf{p}\cdot(\mathbf{x}-\mathbf{x_0})} \\
  &=\left(\frac{m}{2\pi it}\right)^{\frac{3}{2}}
  e^{im(\mathbf{x}-\mathbf{x_0}^2)/2t}.
\end{align*}

\begin{align*}
  U(t) &= \left<\mathbf{x}\left|e^{-it\sqrt{\mathbf{p}^2+m^2}}
  \right| \mathbf{x_0}\right> \\
  &=\frac{1}{(2\pi)^3}\int d^3p e^{-it\sqrt{\mathbf{p}^2+m^2}}\cdot
  e^{i\mathbf{p}\cdot(\mathbf{x}-\mathbf{x_0})} \\
  &=\frac{1}{2\pi^2|\mathbf{x}-\mathbf{x_0}|}
  \int^\infty_0dp\,p\,\sin(p|\mathbf{x}-\mathbf{x_0}|)e^{-it\sqrt{p^2+m^2}}
\end{align*}
\begin{align}
  \lim_{\delta z\rightarrow 0}\frac{\delta f}{\delta z}
  =\lim_{\delta y\rightarrow 0}\frac{\delta u+i\delta v}{i\delta y}
  =-i\frac{\partial u}{\partial y}+\frac{\partial v}{\partial y}
\end{align}
\begin{align}
  \lim_{\delta z\rightarrow 0}\frac{\delta f}{\delta z}
  =\lim_{\delta x\rightarrow 0}\frac{\delta u+i\delta v}{\delta x}
  =\frac{\partial u}{\partial x}+i\frac{\partial v}{\partial x}
\end{align}
\begin{align}
  \int_{z_1}^{z_2}f(z)\,dz = \int_{x_1,y_1}^{x_2,y_2}[u(x,y)+iv(x,y)][dx+idy]
  =\int_{x_1,y_1}^{x_2,y_2}[u(x,y)dx-v(x,y)dy]
  +i\int_{x_1,y_1}^{x_2,y_2}[v(x,y)dx+u(x,y)dy]
\end{align}
\begin{align}
  \oint_C f(z)\,dz=0.
\end{align}
\end{document} 